SATsolver/Experiment/Data/Formula.lean
@@ -6,7 +6,6 @@ namespace Formula
 
 def lits (f : Formula) : List Lit := f.flatten
 
-def wf(f : Formula) : Prop := ∀ c ∈ f, c.wf
 
 def mem_memClause_mem {f : Formula}{c : Clause} :
   c ∈ f → ∀ l ∈ c, l ∈ f.lits := by
@@ -26,6 +25,9 @@ def mem_memClause_mem {f : Formula}{c : Clause} :
 
 
 def names (f : Formula) : List Nat := (f.flatMap Clause.names)
+
+def wf(f : Formula) : Prop := ∀ c ∈ f, c.wf ∧ ∀ n ∈ f.names, ∀ m < n, m ∈ f.names
+
 
 def names_cons {f : Formula}(wf : f.wf) :
   f ≠ [] → f.names ≠ [] := by
@@ -57,6 +59,13 @@ def mem_memClause_mem_names {f : Formula}{c : Clause}{n : Nat} :
       simp[names] at ⊢ this
       right; exact this
 
+def mem_mem_names_cons {tl : Formula}{hd : Clause}{n : Nat} :
+  n ∈ tl.names → n ∈ Formula.names (hd::tl):= by
+  simp[names]
+  intro c cmem nmem
+  right
+  exists c
+
 instance : Membership Clause Formula where
   mem f c := c ∈ f
 
@@ -72,9 +81,55 @@ namespace Variables
 -- Checks that all the variables is in a formula
 -- and that the formula contains all the vars
 def wf (vs : Variables)(f : Formula) : Prop :=
-  (∀ n ∈ f.names, n ≤ vs) ∧ (∀ n ≤ vs, n ∈ f.names)
+  (∀ n ∈ f.names, n ≤ vs) ∧ (∀ n ≤ vs, n ≠ 0 → n ∈ f.names)
+
+theorem f_cons_ne_zero {c : Clause}{cs : Formula}{v : Variables}{fwf : Formula.wf (c::cs)}:
+  v.wf (c::cs) →  v ≠ 0 := by
+  intro vwf
+  simp[Formula.wf, wf, Clause.wf, Formula.names] at *
+  have ⟨ cheq, call, czero⟩ := fwf.1.1
+  simp[List.ne_nil_iff_exists_cons] at cheq
+  obtain ⟨ l, ls, cheq ⟩ := cheq
+  subst cheq
+  simp[Clause.names] at czero
+  have zlt : 0 < l.name := by
+    have := czero.1
+    rw[←Nat.ne_zero_iff_zero_lt]
+    intro contra
+    rw[contra] at this
+    contradiction
+  have lle := vwf.1 l.name (by simp[Clause.names])
+  have : 0 < v := Nat.lt_of_lt_of_le zlt lle
+  simp[Nat.ne_zero_iff_zero_lt, this]
+
 
 instance : DecidableRel wf := by
   intro vs f
   simp[wf]
   exact instDecidableAnd
+
+
+end Variables
+
+
+
+/-
+def exists_v {f : Formula}{wf : f.wf} :
+  f ≠ [] → ∃ (v : Variables), v.wf f := by
+  simp[Variables.wf, Formula.wf] at *
+  intro h
+  induction f
+  case nil => contradiction
+  case cons c cs csih =>
+    cases cs
+    case nil =>
+      simp[Formula.names, Clause.wf] at *
+      induction c
+      case nil => simp at wf
+      case cons l ls lsih =>
+        cases ls
+        case nil =>
+          simp[Clause.names]
+          exists l.name
+          simp
+-/
