SATsolver/Experiment/Data/Trail.lean
@@ -13,8 +13,22 @@ theorem mem_mem_lits{t : Trail}{a : ALit} :
   intro h
   exists a
 
+theorem lits_append(hd tl : Trail):
+  (hd++tl).lits = hd.lits++tl.lits := by
+  simp[lits]
+
+theorem lits_cons (hd: ALit)(tl : Trail):
+  Trail.lits (hd::tl) = hd.lit::tl.lits := by
+  simp[lits]
+
 def names : Trail → List Nat
   |t => t.map ALit.name
+
+theorem mem_mem_names{t : Trail}{a : ALit} :
+  a ∈ t → a.name ∈ t.names := by
+  simp[names]
+  intro h
+  exists a
 
 theorem mem_name_exists_mem {t : Trail}{n : Nat} :
   n ∈ t.names → ∃ a ∈ t, a.name = n := by
@@ -28,6 +42,52 @@ theorem names_cons (hd: ALit)(tl : Trail):
   Trail.names (hd::tl) = hd.name::tl.names := by
   simp[names]
 
+theorem mem_lits_mem_names {t : Trail}{l : Lit} :
+  l ∈ t.lits → l.name ∈ t.names := by
+  simp[lits, names]
+  intro a amem heq
+  exists a
+  have := congrArg Lit.name heq
+  simp[ALit.name_name_lit] at this
+  simp[this, amem]
+
+theorem mem_lits_names_eq {t : Trail}{l : Lit} :
+  l ∈ t.lits ∨ l.negate ∈ t.lits ↔ l.name ∈ t.names := by
+  simp[lits, names]
+  constructor
+  case mp =>
+    intro h
+    cases h
+    case inl lh =>
+      obtain ⟨ a, amem, heq ⟩ := lh
+      exists a
+      constructor
+      case left => exact amem
+      case right => simp[←heq, ALit.name_name_lit]
+    case inr rh =>
+      obtain ⟨ a, amem, heq ⟩ := rh
+      exists a
+      constructor
+      case left => exact amem
+      case right =>
+        have := congrArg Lit.name heq
+        simp[ALit.name_name_lit, Lit.name_name_negate] at this
+        exact this
+  case mpr =>
+    intro h
+    obtain ⟨ a, amem, heq ⟩ := h
+    rw[←ALit.name_name_lit] at heq
+    have := Lit.shared_name heq
+    cases this
+    case inl lh =>
+      left
+      exists a
+    case inr rh =>
+      right
+      exists a
+
+
+
 def unseen (t : Trail)(n : Nat) : Prop := n ∉ t.names
 
 instance : DecidableRel unseen :=
@@ -40,8 +100,21 @@ instance : DecidablePred Trail.wf := by
   simp[wf]
   apply instDecidableAnd
 
-def wf_append{hd tl : Trail}:
+theorem wf_append{hd tl : Trail}:
   (hd++tl).wf → hd.wf ∧ tl.wf := by
   simp[wf, names_append, List.nodup_append]
   intro hdNodup tlNodup nodup nozerohd nozerotl
   simp[hdNodup, tlNodup, nozerohd, nozerotl]
+
+theorem wf_cons{hd : ALit}{tl : Trail}:
+  Trail.wf (hd::tl) → tl.wf := by
+  simp[wf, names_cons, List.nodup_cons]
+  intro hdNodup tlNodup nozerohd nozerotl
+  simp[tlNodup, nozerotl]
+
+theorem wf_hd {hd : ALit}{tl : Trail}:
+  Trail.wf (hd::tl) → hd.name ∉ tl.names := by
+  intro h contra
+  simp[wf, names_cons] at h
+  have := h.1.1
+  contradiction
