SATsolver/Experiment/DPLL/Theorem.lean
@@ -1,0 +1,119 @@
+import SATsolver.Experiment.DPLL.impl
+
+theorem internal_final_state{f: Formula}{v : Variables}{vz : v ≠ 0}{wf : f.wf ∧ v.wf f}{b : Bool}{t t' : Trail}{twf : t.wf ∧ ∀ n ∈ t.names, n ∈ f.names}:
+  internal t f v vz wf twf = (b, t') → t' ⊨ f ∨ b = false := by
+  unfold internal
+  split
+  case isTrue hsat =>
+    simp at hsat ⊢
+    intro bh heq
+    simp[←heq, hsat]
+  case isFalse hsat =>
+    split
+    case isTrue hcon =>
+      split
+      case isTrue exDec =>
+        intro h
+        exact internal_final_state h
+      case isFalse exDec =>
+        simp
+        intro bh th
+        simp[bh]
+    case isFalse hcon =>
+      simp
+      split
+      case isTrue hunit =>
+        intro h
+        exact internal_final_state h
+      case isFalse hunit =>
+        intro h
+        exact internal_final_state h
+termination_by distance t v vz
+decreasing_by
+  have : t.length < v := by
+    rename ¬decide (t⊨f) = true => sat
+    rename ¬decide (t⊭f) = true => con
+    simp at sat con
+    have := Trail.ud_vars twf.1 wf.1 wf.2 twf.2 (Formula.nSatCon_ud sat con)
+    simp[Trail.names] at this
+    exact this
+  exact distance_dec this
+  have : t.length < v := by
+    rename ¬decide (t⊨f) = true => sat
+    rename ¬decide (t⊭f) = true => con
+    simp at sat con
+    have := Trail.ud_vars twf.1 wf.1 wf.2 twf.2 (Formula.nSatCon_ud sat con)
+    simp[Trail.names] at this
+    exact this
+  exact distance_prop this
+  have : t.length ≤ v := Trail.mem_vwf twf.1 twf.2 wf.2
+  exact distance_bc this
+
+theorem DPLL.final_state{f : Formula}{v : Variables}{wf : f.wf ∧ v.wf f}{b : Bool}{t : Trail}:
+DPLL f  v wf = (b, t) → t ⊨ f ∨ b = false := by
+  simp[DPLL]
+  cases f
+  case nil => simp[Satisfies.sat]
+  case cons c cs =>
+    simp
+    exact internal_final_state
+
+
+theorem DPLL.soundness {f : Formula}{v : Variables}{wf : f.wf ∧ v.wf f}{b : Bool}{t : Trail} :
+  DPLL f  v wf = (b, t) → b = true → ∃ (t : Trail), t ⊨ f := by
+  intro h bh
+  have := DPLL.final_state h
+  simp[bh] at this
+  exists t
+
+theorem internal_final_false{f: Formula}{v : Variables}{vz : v ≠ 0}{wf : f.wf ∧ v.wf f}{t t' : Trail}{twf : t.wf ∧ ∀ n ∈ t.names, n ∈ f.names}:
+  internal t f v vz wf twf = (false, t') → ¬ (∃ (t : Trail), t ⊨ f) := by
+  intro h
+  unfold internal at h
+  split at h
+  case isTrue hsat => simp at h
+  case isFalse hsat =>
+    split at h
+    case isTrue hcon =>
+      simp at h
+      split at h
+      case isTrue hexi =>
+        exact internal_final_false h
+      case isFalse hexi =>
+        simp at hexi
+
+
+
+theorem DPLL.completeness {f : Formula}{v : Variables}{wf : f.wf ∧ v.wf f}:
+  (∃ (t : Trail), t ⊨ f) → ∃ (t : Trail), DPLL f v wf = (true, t) := by
+  intro h
+  obtain ⟨ t, tsat ⟩ := h
+  simp[DPLL]
+  split
+  case h_1 => simp
+  case h_2 f wf hd tl wf' =>
+    unfold internal
+    split
+    case isTrue hsat => simp
+    case isFalse hsat =>
+      split
+      case isTrue hcon =>
+        simp[Conflict.con, Trail.lits] at hcon
+        simp[Formula.wf, Clause.wf] at wf'
+        have := wf'.1.1.1.1
+        obtain ⟨ l, ls, lmem ⟩ := List.ne_nil_iff_exists_cons.mp this
+        cases hcon
+        case inl hcon =>
+          simp[lmem] at hcon
+          have := hcon l
+          simp at this
+        case inr hcon =>
+          obtain ⟨ c, cmem, call ⟩ := hcon
+          have := (wf'.1.2 c cmem).1.1
+          obtain ⟨ l, ls, lmem ⟩ := List.ne_nil_iff_exists_cons.mp this
+          simp[lmem] at call
+          have := call l
+          simp at this
+      case isFalse hcon =>
+        simp
+        split
