SATsolver/Experiment/DPLL/backtrack.lean
@@ -71,3 +71,152 @@ theorem bck_preserves_twf {t : Trail}{f : Formula}
     intro n nmem
     rw[heq, Trail.names_append] at tf
     exact tf n (by simp[nmem])
+
+theorem dedwf_tl {f hd a tl} : (∀ (x : ALit), x ∈ hd → ¬x.decidedP) → a.decidedP → Trail.deduction_wf f (hd ++ a :: tl) → Trail.deduction_wf f tl := by
+    intro hdall adec h
+    induction hd
+    case nil =>
+      cases a
+      case decided l =>
+        simp[Trail.deduction_wf] at h
+        exact h
+      case deduced =>
+        simp[ALit.decidedP] at adec
+    case cons hhd hd ih =>
+      have hdall' : ∀ (x : ALit), x ∈ hd → ¬x.decidedP := by
+        intro x xmem
+        exact hdall x (by simp[xmem])
+      have : Trail.deduction_wf f (hd ++ a :: tl) := by
+        cases hhd
+        case decided =>
+          simp[Trail.deduction_wf] at h
+          exact h
+        case deduced =>
+          simp[Trail.deduction_wf] at h
+          exact h.2
+      exact ih this (hdall := hdall')
+
+
+theorem defwf_hd_ded {tl : Trail}{hd a : ALit}{f : Formula} :
+  Trail.wf (hd :: a :: tl ) ∧ (∀ n ∈ Trail.names (hd :: a :: tl ), n ∈ f.names) → f.wf → hd.deducedP → a.decidedP → Trail.deduction_wf f (hd :: (a :: tl)) →
+  hd :: a :: tl ⊭ f →  (∀ hd, hd :: a :: tl ⊭ f ∨ hd :: a :: tl ¿ f ) := by
+  intro twf fwf hdded hdec hded hcu x
+  cases hd
+  case decided => simp[ALit.deducedP] at hdded
+  case deduced l₁ =>
+    cases a
+    case deduced => simp[ALit.decidedP] at hdec
+    case decided l₂ =>
+      simp[Trail.deduction_wf] at hded
+      cases x
+      case decided l =>
+
+
+
+
+
+
+theorem bck_deduction_inv {f : Formula}{t : Trail}(wf : ∃ a ∈ t, a.decidedP)(twf : t.wf)(fwf : f.wf):
+  t.deduction_wf f → t ⊭ f ∨ t ¿ f →  Trail.deduction_wf f (backtrack t wf twf) := by
+  intro h hcon
+  obtain ⟨ hd, tl, a, heq, adec, hdall ⟩  := exists_split_on_prop ALit.decidedP t wf
+  subst heq
+  have bckl : backtrack (hd ++ a :: tl) wf twf = (ALit.deduced a.lit.negate)::tl := backtrack_lemma hdall adec
+  rw[bckl]
+  simp[Trail.deduction_wf]
+  constructor
+  case right => exact dedwf_tl hdall adec h
+  case left =>
+    cases a
+    case deduced l => simp[ALit.decidedP] at adec
+    case decided l =>
+      simp[Lit.negneg, ALit.lit]
+      intro xs
+      induction xs
+      case nil =>
+        induction hd
+        case nil =>
+          simp at hcon
+          cases hcon
+          case inl hcon => left; exact hcon
+          case inr hcon => right; left; exact hcon
+        case cons y ys ih =>
+          have hdall' : (∀ (x : ALit), x ∈ ys → ¬x.decidedP) := by
+            intro x  xmem
+            exact hdall x (by simp[xmem])
+          have wf' : ∃ a, a ∈ ys ++ ALit.decided l :: tl ∧ a.decidedP := by
+            obtain ⟨ a, amem, adec ⟩ := wf
+            simp[List.mem_cons] at amem
+            cases amem
+            case inl heq =>
+              rw[heq] at adec
+              have := hdall y (by simp)
+              contradiction
+            case inr heq =>
+              exists a
+              simp[heq, adec]
+          have twf' : Trail.wf (ys ++ ALit.decided l :: tl) := Trail.wf_cons twf
+          have ded : Trail.deduction_wf f (ys ++ ALit.decided l :: tl) := by
+            cases y
+            case decided => simp[Trail.deduction_wf] at h; exact h
+            case deduced => simp[Trail.deduction_wf] at h; exact h.2
+          have : ys ++ ALit.decided l :: tl⊭f ∨ ys ++ ALit.decided l :: tl¿f := by
+            cases hcon
+            case inl hcon =>
+              exact Trail.cons_con twf fwf hcon
+            case inr hcon =>
+              right; exact Trail.ud_tl_ud twf hcon
+          have bckl' : backtrack (ys ++ ALit.decided l :: tl) wf' twf' = ALit.deduced (ALit.decided l).lit.negate :: tl := by
+            cases y
+            case decided l =>
+              have := hdall (ALit.decided l) (by simp)
+              simp[ALit.decidedP] at this
+            case deduced l =>
+              simp[backtrack] at bckl
+              exact bckl
+          exact ih hdall' wf' twf' ded this bckl'
+      case cons x xs ih =>
+
+
+
+
+
+
+
+
+
+
+theorem bck_deduction_inv {f : Formula}{t : Trail}{wf : ∃ a ∈ t, a.decidedP}{twf : t.wf}:
+  t.deduction_wf f → t ⊭ f →  Trail.deduction_wf f (backtrack t wf twf) := by
+  intro hwf con
+  induction t
+  case nil => simp at wf
+  case cons hd tl ih =>
+    cases hd
+    case decided l =>
+      simp[backtrack, Trail.deduction_wf]
+      constructor
+      case left =>
+        intro hd
+        left
+        have := (Trail.con_cons_con con) hd
+        simp[Lit.negneg, this]
+      case right =>
+        simp[Trail.deduction_wf] at hwf
+        exact hwf
+    case deduced l =>
+      simp[backtrack]
+      have hwf' : Trail.deduction_wf f tl := hwf.2
+      have wf' : ∃ a, a ∈ tl ∧ a.decidedP := by
+        obtain ⟨ a, amem, adec ⟩ := wf
+        cases a
+        case decided k =>
+          simp at amem
+          exists ALit.decided k
+        case deduced k =>
+          simp [ALit.decidedP] at adec
+      have twf' : Trail.wf tl := Trail.wf_cons twf
+      obtain ⟨ hd', tl', a, heq, adec,hall⟩  := exists_split_on_prop ALit.decidedP tl wf'
+      subst heq
+      have : backtrack (hd' ++ a :: tl') wf' twf' = ALit.deduced (a.lit.negate)::tl' := backtrack_lemma hall adec
+      rw[this]
