SATsolver/Experiment/DPLL/propogate.lean
@@ -16,7 +16,7 @@ theorem ppg_preserves_wf {t : Trail}{c : Clause}{cu : c.unit t}{f : Formula}
   case left =>
     have : 0 ≠ (c.getunit t cu).name := by
       intro contra
-      simp[←contra, (fwf c cmem).2.2] at unit_name_mem
+      simp[←contra, (fwf c cmem).1.2.2] at unit_name_mem
     simp[propogate, List.nodup_cons, Trail.names_cons, twf, ALit.name, unit_ud, this]
   case right =>
     intro n nmem
@@ -26,3 +26,52 @@ theorem ppg_preserves_wf {t : Trail}{c : Clause}{cu : c.unit t}{f : Formula}
       have := Formula.mem_memClause_mem_names cmem unit_name_mem
       simp[ALit.name, this]
     case tail mem => exact twf.2 n mem
+
+theorem ppg_negation_con {l : Lit} {t : Trail}{c : Clause}{cu : c.unit t}{f : Formula}:
+  propogate t c cu = ALit.deduced l :: t → c ∈ f → ALit.decided l.negate :: t ⊭ f := by
+  intro h hmem
+  simp[propogate] at h
+  have lmem : l ∈ c := by
+    rw[←h]
+    exact Clause.unit_mem
+  have lud : t ¿ l := by
+    rw[←h]
+    exact Clause.unit_ud
+  simp[Clause.unit] at cu
+  obtain ⟨ k, kmem, kud, kall ⟩ := cu
+  by_cases heq : l = k
+  case neg =>
+    have := kall l lmem heq
+    simp[Conflict.con, Undecided.ud] at lud this
+    have := Trail.mem_lits_mem_names this
+    simp[Lit.name_name_negate] at this
+    contradiction
+  case pos =>
+    simp[Conflict.con] at kall ⊢
+    exists c
+    simp[hmem]
+    intro j jmem
+    by_cases heq2 : j = k
+    case pos =>
+      rw[heq2, heq]
+      simp[Trail.lits, ALit.lit]
+    case neg =>
+      have := kall j jmem heq2
+      simp[Trail.lits_cons, this]
+
+theorem ppg_deduction_inv {t : Trail}{c : Clause}{cu : c.unit t}{f : Formula}:
+  t.deduction_wf f → c ∈ f → Trail.deduction_wf f (propogate t c cu) := by
+  intro h cmem
+  let l := c.getunit t cu
+  have : propogate t c cu = ALit.deduced l :: t := by
+    simp[propogate, l]
+  rw[this]
+  simp[Trail.deduction_wf]
+  have := ppg_negation_con this cmem
+  constructor
+  case left =>
+    intro hd
+    left
+    exact (Trail.con_cons_con this) hd
+  case right =>
+    exact h
